beluga_clean/progress.v
@@ -1,5 +1,62 @@
 Require Import divergence.
 Require Import subj_red.
+Set Implicit Arguments.
+
+Inductive val {δ γ} : checked_exp δ γ -> Prop :=
+| val_var : forall x, val (var δ x)
+| val_tt : val tt
+| val_fold : forall E, val E -> val (fold E)
+| val_inl : forall E, val E -> val (inl E)
+| val_inr : forall E, val E -> val (inr E)
+| val_pair : forall E1 E2, val E1 -> val E2 -> val (pair E1 E2)
+| val_pack : forall E C, val E -> val (pack C E)
+| val_fn : forall δ' γ' γ'' (y:γ'↪γ'') (E:checked_exp δ' γ'') θ ρ,
+           val ((fn y E)[θ;;ρ])
+| val_mlam : forall δ' δ'' γ' (X:δ'↪δ'')(E:checked_exp δ'' γ') θ ρ,
+           val ((mlam X E)[θ;;ρ])
+| val_meta : forall C, val (meta _ C)
+.
+
+Hint Constructors val.
+Lemma eval_to_val E V : E ⇓ V -> val V.
+induction 1; eauto. inversion IHeval. eauto.
+Qed.
+
+Inductive canonical : checked_exp ∅ ∅ -> tp ∅ -> Prop :=
+| canon_fn : forall δ γ γ' (y:γ↪γ') (E:checked_exp δ γ') θ ρ T S,
+                 canonical ((fn y E)[θ;;ρ]) (arr T S)
+| canon_mlam : forall δ δ' γ (X:δ↪δ') (E:checked_exp δ' γ) θ ρ U T,
+                 canonical ((mlam X E)[θ;;ρ]) (pi ₁ U T)
+| canon_fold : forall ψ δ (Z:∅↪ψ) (X:∅↪δ) E C U T,
+                 canonical (fold E) (tapp (mu Z X U T) C)
+| canon_tt : canonical tt unit
+| canon_inl : forall E T S, canonical (inl E) (sum T S)
+| canon_inr : forall E T S, canonical (inr E) (sum T S)
+| canon_pair : forall E1 E2 T S, canonical (pair E1 E2) (prod T S)
+| canon_pack : forall δ (X:∅↪δ) C E U T,
+                  canonical (pack C E) (sigma X U T)
+| canon_meta : forall C U, canonical (meta _ C) (m_tp' U)
+.
+
+Hint Constructors canonical.
+
+Lemma canonical_forms V T : val V -> ·;· ⊢ V ⇐ T -> canonical V T.
+intros. nice_inversion H; invert_typing; simpl; eauto.
+edestruct empty_is_empty; eauto.
+Qed.
+
+Lemma canonical_forms' δ γ θ ρ (E:checked_exp δ γ) V :
+   E[θ;;ρ] ⇓ V
+-> forall Δ Γ, (· ⊩ θ ∷ Δ)
+-> (·;· ⊪ ρ ⇐ (〚θ〛 ○ Γ))
+-> forall T, Δ;Γ ⊢ E ⇐ T
+-> canonical V (〚θ〛T).
+intros.
+eapply canonical_forms.
+eapply eval_to_val; eauto.
+eapply subj_red; eauto.
+Qed.
+Hint Resolve canonical_forms'.
 
 Axiom classical : forall P, P \/ ~P.
 
@@ -26,12 +83,19 @@ admit. (* TODO *)
 (* app *)
 doesItConverge (I0[θ;;ρ]).
 doesItConverge (E[θ;;ρ]).
-clear progress. admit. (* TODO: Eval to val, canonical forms *)
+assert (canonical V (〚θ〛(arr T1 T0))) as Hy by eauto.
+  nice_inversion Hy.
+
+doesItConverge (E0[θ0;;(ρ0,,(y,V0))]).
+edestruct H0. by eauto.
+eapply div_app3; eauto. 
+(* eapply progress; eauto. *) admit. (* TODO *)
 eapply div_app2; eauto 7.
 eapply div_app1; eauto 7.
 
 (* mapp *)
 doesItConverge (I0[θ;;ρ]).
+
 clear progress. admit. (* TODO *)
 eapply div_mapp1; eauto 7.
 
@@ -45,7 +109,9 @@ eapply H0; eauto.
 econstructor.
 eapply progress; eauto.
 intros v Hy.
-clear progress. admit. (* TODO: Canonical forms *)
+assert (canonical v (〚θ〛(tapp (mu Z X U T) C))) as Hy0 by eauto. (* TODO: Auto *)
+  nice_inversion Hy0.
+eapply H0; by eauto.
 
 (* meta *)
 edestruct H0; by eauto.
